%================================================
%::::::::::::::::::::::::::::::::::::::::::::::::
\chapter{Directional and Partial Derivatives}



\section{Basic Definitions}
%================================================
%------------------------------------------------


%------------------------------------------------
\begin{definition}
	\label{def: directional derived function}
	Let $U$ be an open set in $\mathbb R^m$, and let $f: U \to \mathbb R^n$.

	Let $\vec u \in U$, then the \textit{$\vec u$-directional derived function of $f$} is defined to be
	$$
	\begin{aligned}
		\nabla_{\vec u} f : U \to \mathbb R^n
		&: \vec x \mapsto
		\begin{cases}
			\displaystyle \lim_{t \to 0} \frac{f(\vec x + t \vec u) - f(\vec u)}{t} & \text{, if the limit exists;} \\
			0 & \text{, otherwise.}
		\end{cases}
	\end{aligned}
	$$
	
	The value $\nabla_{\vec u} f(\vec p)$ is called \textit{$\vec u$-directional derivative of $f$ at a point $\vec p \in U$}.
\end{definition}
%------------------------------------------------


%------------------------------------------------
\begin{lemma}
	\label{lm: directional derivad function}
	$$
	\nabla_{\vec u} f = \frac{\mathrm d g}{\mathrm d t}
	$$
	
	\begin{proof}
		By Definition \ref{def: directional derived function}, we have
		$$
		\nabla
		$$
	\end{proof}
\end{lemma}
%------------------------------------------------



%------------------------------------------------
\begin{proposition}
	$$
	\nabla_{s \vec u} f = s \nabla_{\vec u} f.
	$$
	
	\begin{proof}
		By Definition \ref{def: directional derived function}, we have
		$$
		\nabla_{s\vec u} f(\vec x) = \lim_{t \to 0} \frac{f(\vec x + t s \vec u) - f(\vec x)}{t}.
		$$
		
		Now, fix $\vec x$, and define
		$$
		g(t) := f(\vec x + t \vec u),
		$$
		then we have
		$$
		\begin{aligned}
			\nabla_{s \vec u} f(\vec x) &= \lim_{t \to 0} \frac{g(s t) - g(0)}{t} \\
			&= \left. \frac{\mathrm d g(st)}{\mathrm d t} \right|_{t = 0} \\
			&= \left. \frac{\mathrm d g(st)}{\mathrm d st} \cdot \frac{\mathrm dst}{\mathrm d t} \right|_{t = 0} \\
			&= s \cdot \left. \frac{\mathrm d g(t)}{\mathrm d t} \right|_{t = 0} \\
			&= s \cdot \lim_{t \to 0} \frac{f(\vec x + t \vec u) - f(\vec x)}{t} \\
			&= s \nabla_{\vec u} f(\vec x).
		\end{aligned}
		$$
	\end{proof}
\end{proposition}
%------------------------------------------------












%------------------------------------------------
%================================================






























%::::::::::::::::::::::::::::::::::::::::::::::::
%================================================
